\subsection{Example~1.12}

We have for every two points~$y$ and~$z$ in~$X$ the (in)equalities
\[
	f y
	=
	d(x, y)
	≤
	d(x, z) + d(z, y)
	=
	f z + d(y, z) \,,
\]
and therefore the inequality
\[
	f y - f z ≤ d(y, z) \,.
\]
By swapping the roles of~$y$ and~$z$ we get also the inequality
\[
	f z - f y ≤ d(z, y) = d(y, z) \,.
\]
We can combine both of these inequalities into the single inequality
\[
	\abs{f y - f z} ≤ d(y, z) \,.
\]
This inequality tells us that the function~$f$ is Lipschitz continuous, and therefore continuous.
