\subsection{Pushforward of Filters}

An alternative construction of pushforwards of filters is given as follows.

\begin{proposition}
	Let~$X$ and~$Y$ be two sets and let~$f$ be a map from~$X$ to~$Y$.
	Let~$\filter{F}$ be a filter on~$X$.
	Then $f_* \filter{F} â‰” \{ B âŠ† Y \suchthat f^{-1} B âˆˆ \filter{F}\}$ is a filter on~$Y$.
\end{proposition}

\begin{proof}[First proof]
	We have~$f^{-1} Y = X âˆˆ \filter{F}$, and therefore~$Y âˆˆ f_* \filter{F}$.
	We have for every two subsets~$A$ and~$B$ of~$X$ the chain of equivalences
	\begin{align*}
		{}&
		A âˆ© B âˆˆ f_* \filter{F} \\
		\iff{}&
		f^{-1} (A âˆ© B) âˆˆ \filter{F} \\
		\iff{}&
		f^{-1} A âˆ© f^{-1} B âˆˆ \filter{F} \\
		\iff{}&
		f^{-1} A, f^{-1} B âˆˆ \filter{F} \\
		\iff{}&
		A, B âˆˆ f_* \filter{F} \,.
	\end{align*}
	According to \cref{slick criterion for filters}, this shows that~$\filter{F}$ is a filter on~$Y$.
\end{proof}

\begin{proof}[Second proof]
	The given filter~$\filter{F}$ corresponds to a homomorphism of meet-semilattices~$Ï‡$ from~$2^X$ to~$ğŸ™$ with~$\filter{F} = Ï‡^{-1} 1$.
	The map~$f$ induces a map~$f^â™¯$ from~$2^Y$ to~$2^X$ that assigns to each subset of~$Y$ its preimage under~$f$.
	This map~$f^â™¯$ is a homomorphism of meet-semilattices since~$f^â™¯ Y = f^{-1} Y = X$ and
	\[
		f^â™¯ (A âˆ© B)
		=
		f^{-1} (A âˆ© B)
		=
		f^{-1} A âˆ© f^{-1} B
		=
		f^â™¯ A âˆ© f^â™¯ B
	\]
	for any two subsets~$A$ and~$B$ of~$Y$.
	The composite~$Ï‡ f^â™¯$ is a homomorphism of meet-semilattices from~$2^Y$ to~$ğŸš$.
	This homomorphism corresponds to a filter on~$Y$, given by
	\begin{align*}
		(Ï‡ f^â™¯)^{-1} 1
		=
		(f^â™¯)^{-1} Ï‡^{-1} 1
		=
		(f^â™¯)^{-1} \filter{F}
		&=
		\{ B âŠ† Y \suchthat f^â™¯ B âˆˆ \filter{F} \} \\
		&=
		\{ B âŠ† Y \suchthat f^{-1} B âˆˆ \filter{F} \} \,.
	\end{align*}
	This filter is precisely~$f_* \filter{F}$, which is therefore a filter.
\end{proof}

Our construction agrees with the one from Definition~3.6:
we have for the filter~$\filter{G}$ generated by the set~$\{ f A \suchthat A âˆˆ \filter{F} \}$ the chain of equalities
\begin{align*}
	\filter{G}
	&=
	\{ B âŠ† Y \suchthat \text{there exists~$A âˆˆ \filter{F}$ with~$f A âŠ† B$} \} \\
	&=
	\{ B âŠ† Y \suchthat \text{there exists~$A âˆˆ \filter{F}$ with~$A âŠ† f^{-1} B$} \} \\
	&=
	\{ B âŠ† Y \suchthat f^{-1} B âˆˆ \filter{F} \} \\
	&=
	f_* \filter{F} \,.
\end{align*}
