\subsection{Exercise 0.6}

Let~$η$ be a natural transformation from~$\cat{C}(\ph, X)$ to~$F$.
The component~$η_X$ is a map from~$\cat{C}(X, X)$ to~$F X$.
We can therefore consider the element~$η_X \id_X$ of~$F X$.

We observe that the entire natural transformation~$η$ is already determined by the single element~$η_X \id_X$:
we have for every object~$Y$ of~$\cat{C}$ and every element~$f$ of~$\cat{C}(Y, X)$ the chain of equalities
\[
	η_Y f
	=
	η_Y f^* \id_X
	=
	(F f) η_X \id_X \,.
\]

Suppose on the other hand that~$x$ is any element of~$F X$.
For every object~$Y$ of~$\cat{C}$ we consider the map
\[
	η_Y
	\colon
	\cat{C}(Y, X) \to F Y \,,
	\quad
	g \mapsto (F g) x \,.
\]
The resulting transformation~$η$ from~$\cat{C}(\ph, X)$ to~$F$ is natural.
To prove this, we need to check that for every morphism~$f \colon Y \to Z$ the square
\[
	\begin{tikzcd}
		\cat{C}(Z, X)
		\arrow{r}[above]{f^*}
		\arrow{d}[left]{η_Z}
		&
		\cat{C}(Y, X)
		\arrow{d}[right]{η_Y}
		\\
		F Z
		\arrow{r}[above]{F(f)}
		&
		F Y
	\end{tikzcd}
\]
commutes.
This commutativity holds because for every element~$g$ of the top-left corner we have the chain of equalities
\[
	η_Y f^* g
	=
	η_Y (g f)
	=
	F(g f)(x)
	=
	F(f) F(g) x
	=
	F(f) η_Z g \,.
\]
The constructed natural transformation~$η$ satisfies
\[
	η_X \id_X
	=
	(F \id_X) x
	=
	\id_{F X} x
	=
	x \,.
\]
