\subsection*{Theorem 0.1}

It remains to show that the third bullet point is equivalent to the previous two ones.

We note that for every morphism~$f \colon X \to Y$ in~$\cat{C}$, the pullback
\[
	f^* \colon \cat{C}(Y, Z) \to \cat{C}(X, Z)
\]
is the same as the push-forward
\[
	f_* \colon \cat{C}^{\op}(Z, Y) \to \cat{C}^{\op}(Z, X) \,.
\]
We also note that a morphism~$g \colon Y \to X$ is an inverse for~$f$ in~$\cat{C}$ if and only if it is an inverse for~$f$ in~$\cat{C}^{\op}$;
therefore,~$f$ is an isomorphism in~$\cat{C}$ if and only if it is an isomorphism in~$\cat{C}^{\op}$.

We now find from the already proven equivalence that
\begin{align*}
	{}&
	\text{$f$ is an isomorphism in~$\cat{C}$}
	\\
	\iff{}&
	\text{$f$ is an isomorphism in~$\cat{C}^{\op}$}
	\\
	\iff{}&
	\text{$f_* \colon \cat{C}^{\op}(Z, Y) \to \cat{C}^{\op}(Z, X)$ is an isomorphism for every~$Z$}
	\\
	\iff{}&
	\text{$f^* \colon \cat{C}(Y, Z) \to \cat{C}(X, Z)$ is an isomorphism for every~$Z$} \,.
\end{align*}
